\section{Integração de Romberg}

Suponha que $I_{n}$ seja o resultado da integração pela regra do trapézio estendida com \esp{k = \displaystyle \frac{(b-a)}{N}}

Suponha que $I_{2n}$ seja o resultado para \esp{ \overline{h} = \displaystyle \frac{(b-a)}{(N/2)} }.

Assim,

\begin{equation}
 \label{cap2:sec4:eq1}
 E_h \approx - \frac{1}{12} \, (b-a) \, \overline{f}'' \, h^2 \approx C\,h^2
\end{equation}

\begin{equation}
 \label{cap2:sec4:eq2}
 E_{2\,h} \approx - \frac{1}{12} \, (b-a) \, \overline{f}'' \, (2\,h)^2 \approx 4\,C\,h^2
\end{equation}

A integral exata é

\begin{equation}
 \label{cap2:sec4:eq3}
I = I_h + E_h = I_{2\,h} + E_{2\,h}
\end{equation}

Assim,

\begin{equation}
 \label{cap2:sec4:eq4}
 E_h - E_{2\,h} = I_{2\,h} - I_h
\end{equation}

Eq. \ref{cap2:sec4:eq1} e \ref{cap2:sec4:eq2} $ \rightarrow $ \ref{cap2:sec4:eq4} $ \Rightarrow $

\[
 \begin{array}{ll}
              & C\,h^2 - 4\,C\,h^2 = I_{2\,h} - I_h \\
  \Rightarrow & C = \displaystyle \frac{1}{3} \, h^{-2} \, (I_h - I_{2\,h})
 \end{array}
\]

\[
 E_h \approx \frac{1}{3} \, (I_h - I_{2\,h})
\]

\[
 \quadricular{ I = I_h + E_h \approx I_h + \frac{1}{3} \, (I_h - I_{2\,h}) }
\]

\begin{example}

\[
 \begin{array}{ll}
  I_{0.5} = 11.9895 \qquad \qquad & I_{0.25} = 11.7940 \\
  \uparrow & \uparrow \\
  N = 2 & N = 4 \\
  \\
  h = 0.25
 \end{array}
\]

\[
 \begin{array}{lc}
  I = 11.7940 + \displaystyle \frac{1}{3} \, (11.7940 - 11.9895) & \approx 11.7288 \\
  & \uparrow \\
  & \approx I_{0.0156} \\
  & \uparrow \\
  & N = 128
 \end{array}
\]

\end{example}